src/lib/data/Kuiper.Matrix.Reprs.Type.fsti
@@ -27,6 +27,9 @@ let full_mlayout (rows cols : nat) =
 let mlayout_size (#rows #cols : nat) (l : mlayout rows cols) : GTot nat =
   l.len
 
+let mlayout_vsize (#rows #cols : nat) (_l : mlayout rows cols) : GTot nat =
+  rows * cols
+
 inline_for_extraction
 type mrepr = rows:nat -> cols:nat -> full_mlayout rows cols
 
